Refactor incarnations in to separate module

src/Verifier/Verifier.dfy
@@ -3,6 +3,7 @@ module Verifier {
   import opened Basics
   import opened Ast
   import opened SolverExpr
+  import I = Incarnations
   import RSolvers
   import StaticConsistency
   import AssignmentTargets
@@ -33,12 +34,12 @@ module Verifier {
     {
       var func: Function :| func in funcs;
       funcs := funcs - {func};
-      var inputTypes := SeqMap(func.Parameters, (parameter: FParameter) => DeclMappings.Type2STypeWithMap(parameter.typ, typeMap));
-      var f := new SVar.Function(func.Name, inputTypes, DeclMappings.Type2STypeWithMap(func.ResultType, typeMap));
+      var inputTypes := SeqMap(func.Parameters, (parameter: FParameter) => I.DeclMappings.Type2STypeWithMap(parameter.typ, typeMap));
+      var f := new SVar.Function(func.Name, inputTypes, I.DeclMappings.Type2STypeWithMap(func.ResultType, typeMap));
       functionMap := functionMap[func := f];
     }
 
-    var declMap := DeclMappings(typeMap, functionMap);
+    var declMap := I.DeclMappings(typeMap, functionMap);
     var procs := b3.procedures;
     while procs != {}
     {
@@ -50,7 +51,7 @@ module Verifier {
     }
   }
 
-  method VerifyProcedure(proc: Ast.Procedure, declMap: DeclMappings)
+  method VerifyProcedure(proc: Ast.Procedure, declMap: I.DeclMappings)
     requires proc.WellFormed()
   {
     var smtEngine := RSolvers.CreateEngine();
@@ -71,10 +72,10 @@ module Verifier {
     CheckAExprs(proc.Post, bodyIncarnations, context, smtEngine, "postcondition");
   }
 
-  method CreateProcIncarnations(parameters: seq<Parameter>, declMap: DeclMappings) returns (preIncarnations: Incarnations, bodyIncarnations: Incarnations)
+  method CreateProcIncarnations(parameters: seq<Parameter>, declMap: I.DeclMappings) returns (preIncarnations: I.Incarnations, bodyIncarnations: I.Incarnations)
     requires forall i :: 0 <= i < |parameters| ==> parameters[i].WellFormed()
   {
-    preIncarnations, bodyIncarnations := Incarnations.Empty(declMap), Incarnations.Empty(declMap);
+    preIncarnations, bodyIncarnations := I.Incarnations.Empty(declMap), I.Incarnations.Empty(declMap);
     for i := 0 to |parameters| {
       var parameter := parameters[i];
       match parameter.mode
@@ -93,117 +94,7 @@ module Verifier {
     }
   }
 
-  type RExpr = RSolvers.RExpr
-
-  datatype DeclMappings = DeclMappings(typeMap: map<Types.TypeDecl, STypeDecl>, functionMap: map<Function, STypedDeclaration>)
-  {
-    function Type2SType(typ: Type): SType {
-      Type2STypeWithMap(typ, typeMap)
-    }
-
-    static function Type2STypeWithMap(typ: Type, typeMap: map<Types.TypeDecl, STypeDecl>): SType {
-      match typ
-      case BoolType => SBool
-      case IntType => SInt
-      case UserType(decl) =>
-        assume {:axiom} decl in typeMap;
-        var sTypeDecl := typeMap[decl];
-        SUserType(sTypeDecl)
-    }
-  }
-
-  datatype Incarnations = Incarnations(nextSequenceCount: map<string, nat>, m: map<Variable, SVar>, declMap: DeclMappings)
-  {
-    static function Empty(declMap: DeclMappings): Incarnations {
-      Incarnations(map[], map[], declMap)
-    }
-
-    function Variables(): set<Variable> {
-      m.Keys
-    }
-
-    // `Set` is intended to be used only during custom initializations of an Incarnations.
-    function Set(v: Variable, sv: SVar): Incarnations {
-      this.(nextSequenceCount := map[v.name := 0] + nextSequenceCount, m := m[v := sv])
-    }
-
-    method Update(v: Variable) returns (incarnations: Incarnations, x: SVar) {
-      var name := v.name;
-      var nextSequenceNumber;
-      if name in nextSequenceCount.Keys {
-        var n := nextSequenceCount[name];
-        name := name + "%" + Int2String(n);
-        nextSequenceNumber := n + 1;
-      } else {
-        nextSequenceNumber := 0;
-      }
-      x := new SVar(name, declMap.Type2SType(v.typ));
-      incarnations := this.(nextSequenceCount := nextSequenceCount[v.name := nextSequenceNumber], m := m[v := x]);
-    }
-
-    function DomainRestrict(variables: set<Variable>): Incarnations {
-      var m' := map v <- m.Keys | v in variables :: m[v];
-      this.(m := m')
-    }
-
-    function REval(expr: Expr): RSolvers.RExpr
-      requires expr.WellFormed()
-    {
-      match expr
-      case BLiteral(value) => RExpr.Boolean(value)
-      case ILiteral(value) => RExpr.Integer(value)
-      case CustomLiteral(s, typ) => RExpr.CustomLiteral(s, declMap.Type2SType(typ))
-      case IdExpr(v) =>
-        assume {:axiom} v in m; // TODO: it would be nice to be able to keep the original variable if there's no incarnation; that would be the case for the bound variable in a let expression or quantifier
-        RExpr.Id(m[v])
-      case OperatorExpr(op, args) =>
-        var rArgs := REvalList(args);
-        match op {
-          case IfThenElse =>
-            RExpr.IfThenElse(rArgs[0], rArgs[1], rArgs[2])
-          case Neq =>
-            var eq := RExpr.FuncAppl(RExpr.Operator2ROperator(Operator.Eq), rArgs);
-            RExpr.FuncAppl(RExpr.Operator2ROperator(Operator.LogicalNot), [eq])
-          case _ =>
-            RExpr.FuncAppl(RExpr.Operator2ROperator(op), rArgs)
-        }
-      case FunctionCallExpr(func, args) =>
-        var rArgs := REvalList(args);
-        assume {:axiom} func in declMap.functionMap;
-        RExpr.FuncAppl(RSolvers.UserDefinedFunction(declMap.functionMap[func]), rArgs)
-      case LabeledExpr(_, body) =>
-        // TODO: do something with the label
-        REval(body)
-      case LetExpr(v, rhs, body) =>
-        RExpr.Boolean(true) //RExpr.LetExpr(v, REval(rhs), REval(body)) // TODO: this requires RExpr and Expr have the same Variables.
-      case QuantifierExpr(univ, v, patterns, body) =>
-        var trs := REvalPatterns(patterns);
-        var b := REval(body);
-        RExpr.Boolean(true) //RExpr.QuantifierExpr(univ, v, trs, b) // TODO: this requires RExpr and Expr have the same Variables.
-    }
-
-    function REvalList(exprs: seq<Expr>): seq<RSolvers.RExpr>
-      requires forall expr <- exprs :: expr.WellFormed()
-      ensures |REvalList(exprs)| == |exprs|
-    {
-      if exprs == [] then
-        []
-      else
-        [REval(exprs[0])] + REvalList(exprs[1..])
-    }
-
-    function REvalPatterns(patterns: seq<Pattern>): seq<seq<RSolvers.RExpr>>
-      requires forall tr <- patterns :: tr.WellFormed()
-    {
-      if patterns == [] then
-        []
-      else
-        assert patterns[0].WellFormed();
-        [REvalList(patterns[0].exprs)] + REvalPatterns(patterns[1..])
-    }
-  }
-
-  method Process(stmts: seq<Stmt>, incarnations_in: Incarnations, context_in: RSolvers.RContext, B: BC.T, smtEngine: RSolvers.REngine)
+  method Process(stmts: seq<Stmt>, incarnations_in: I.Incarnations, context_in: RSolvers.RContext, B: BC.T, smtEngine: RSolvers.REngine)
     requires forall stmt <- stmts :: stmt.WellFormed()
     requires BC.Valid(B)
     requires smtEngine.Valid()
@@ -225,7 +116,7 @@ module Verifier {
       incarnations, sv := incarnations.Update(v);
       if init.Some? {
         var sRhs := incarnations.REval(init.value);
-        context := RSolvers.Extend(context, RExpr.Eq(RExpr.Id(sv), sRhs));
+        context := RSolvers.Extend(context, RSolvers.RExpr.Eq(RSolvers.RExpr.Id(sv), sRhs));
       }
       BC.StmtMeasurePrepend(body, cont);
       Process([body] + cont, incarnations, context, B, smtEngine);
@@ -233,7 +124,7 @@ module Verifier {
       var sRhs := incarnations.REval(rhs);
       var sLhs;
       incarnations, sLhs := incarnations.Update(lhs);
-      context := RSolvers.Extend(context, RExpr.Eq(RExpr.Id(sLhs), sRhs));
+      context := RSolvers.Extend(context, RSolvers.RExpr.Eq(RSolvers.RExpr.Id(sLhs), sRhs));
       Process(cont, incarnations, context, B, smtEngine);
     case Block(stmts) =>
       BC.AboutStmtSeqMeasureConcat(stmts, cont);
@@ -242,15 +133,17 @@ module Verifier {
       print "UNHANDLED STATEMENT: Call\n"; // TODO
       Process(cont, incarnations, context, B, smtEngine);
     case Check(cond) =>
-      ProveAndReport(context, incarnations.REval(cond), "check", cond, smtEngine);
+      var rCond := incarnations.REval(cond);
+      ProveAndReport(context, rCond, "check", cond, smtEngine);
       Process(cont, incarnations, context, B, smtEngine);
     case Assume(cond) =>
-      context := RSolvers.Extend(context, incarnations.REval(cond));
+      var rCond := incarnations.REval(cond);
+      context := RSolvers.Extend(context, rCond);
       Process(cont, incarnations, context, B, smtEngine);
     case Assert(cond) =>
-      var e := incarnations.REval(cond);
-      ProveAndReport(context, e, "assert", cond, smtEngine);
-      context := RSolvers.Extend(context, e);
+      var rCond := incarnations.REval(cond);
+      ProveAndReport(context, rCond, "assert", cond, smtEngine);
+      context := RSolvers.Extend(context, rCond);
       Process(cont, incarnations, context, B, smtEngine);
     case AForall(v, body) =>
       var bodyIncarnations, _ := incarnations.Update(v);
@@ -259,7 +152,8 @@ module Verifier {
 
       expect !StaticConsistency.ContainsNonAssertions(stmt); // TODO: prove that this follows from the AForall statement satisfying its static checks
       var L := Learn(stmt);
-      context := RSolvers.Extend(context, incarnations.REval(L));
+      var rL := incarnations.REval(L);
+      context := RSolvers.Extend(context, rL);
       Process(cont, incarnations, context, B, smtEngine);
     case Choice(branches) =>
       for i := 0 to |branches|
@@ -289,11 +183,12 @@ module Verifier {
       }
       Process(cont, incarnations', context, B0, smtEngine);
     case Probe(e) =>
-      context := RSolvers.Record(context, incarnations.REval(e), incarnations.declMap.Type2SType(e.ExprType()));
+      var rExpr := incarnations.REval(e);
+      context := RSolvers.Record(context, rExpr, incarnations.Type2SType(e.ExprType()));
       Process(cont, incarnations, context, B, smtEngine);
   }
 
-  method ProcessLoop(stmt: Stmt, incarnations_in: Incarnations, context_in: RSolvers.RContext, B: BC.T, smtEngine: RSolvers.REngine)
+  method ProcessLoop(stmt: Stmt, incarnations_in: I.Incarnations, context_in: RSolvers.RContext, B: BC.T, smtEngine: RSolvers.REngine)
     requires stmt.Loop? && stmt.WellFormed() && BC.Valid(B) && smtEngine.Valid()
     modifies smtEngine.Repr
     ensures smtEngine.Valid()
@@ -329,7 +224,7 @@ module Verifier {
     CheckAExprs(stmt.invariants, incarnations, context, smtEngine, "invariant maintained");
   }
 
-  method CheckAExprs(aexprs: seq<AExpr>, incarnations: Incarnations, context: RSolvers.RContext, smtEngine: RSolvers.REngine, errorText: string)
+  method CheckAExprs(aexprs: seq<AExpr>, incarnations: I.Incarnations, context: RSolvers.RContext, smtEngine: RSolvers.REngine, errorText: string)
     requires forall ae <- aexprs :: ae.WellFormed()
     requires smtEngine.Valid()
     modifies smtEngine.Repr
@@ -341,12 +236,13 @@ module Verifier {
       assert aexprs[i].WellFormed();
       match aexprs[i]
       case AExpr(e) =>
-        ProveAndReport(context, incarnations.REval(e), errorText, e, smtEngine);
+        var rExpr := incarnations.REval(e);
+        ProveAndReport(context, rExpr, errorText, e, smtEngine);
       case _ => // TODO
     }
   }
 
-  method AssumeAExprs(aexprs: seq<AExpr>, incarnations: Incarnations, context_in: RSolvers.RContext, smtEngine: RSolvers.REngine)
+  method AssumeAExprs(aexprs: seq<AExpr>, incarnations: I.Incarnations, context_in: RSolvers.RContext, smtEngine: RSolvers.REngine)
       returns (context: RSolvers.RContext)
     requires forall ae <- aexprs :: ae.WellFormed()
     requires smtEngine.Valid()
@@ -360,7 +256,8 @@ module Verifier {
       assert aexprs[i].WellFormed();
       match aexprs[i]
       case AExpr(e) =>
-        context := RSolvers.Extend(context, incarnations.REval(e));
+        var rExpr := incarnations.REval(e);
+        context := RSolvers.Extend(context, rExpr);
       case _ => // TODO
     }
   }
@@ -368,7 +265,7 @@ module Verifier {
   // `errorReportingInfo` is currently an expression that, together with `errorText`, gets printed
   // if `context ==> expr` cannot be proved by `smtEngine`.
   // TODO: This should be improved to instead use source locations.
-  method ProveAndReport(context: RSolvers.RContext, expr: RExpr, errorText: string, errorReportingInfo: Expr, smtEngine: RSolvers.REngine)
+  method ProveAndReport(context: RSolvers.RContext, expr: RSolvers.RExpr, errorText: string, errorReportingInfo: Expr, smtEngine: RSolvers.REngine)
     requires smtEngine.Valid()
     modifies smtEngine.Repr
     ensures smtEngine.Valid()
