src/Verifier/Incarnations.dfy
@@ -1,0 +1,140 @@
+module Incarnations {
+  import opened Basics
+  import opened Ast
+  import opened SolverExpr
+  import Types
+  import RSolvers
+
+  export
+    reveals DeclMappings
+    provides DeclMappings.Type2SType, DeclMappings.Type2STypeWithMap
+    provides Incarnations
+    provides Incarnations.Empty, Incarnations.Set, Incarnations.Update, Incarnations.Variables, Incarnations.DomainRestrict
+    provides Incarnations.REval, Incarnations.Type2SType
+    provides Types, Ast, SolverExpr, RSolvers
+
+  type RExpr = RSolvers.RExpr
+
+  datatype DeclMappings = DeclMappings(typeMap: map<Types.TypeDecl, STypeDecl>, functionMap: map<Function, STypedDeclaration>)
+  {
+    function Type2SType(typ: Type): SType {
+      Type2STypeWithMap(typ, typeMap)
+    }
+
+    static function Type2STypeWithMap(typ: Type, typeMap: map<Types.TypeDecl, STypeDecl>): SType {
+      match typ
+      case BoolType => SBool
+      case IntType => SInt
+      case UserType(decl) =>
+        assume {:axiom} decl in typeMap;
+        var sTypeDecl := typeMap[decl];
+        SUserType(sTypeDecl)
+    }
+  }
+
+  datatype Incarnations = Incarnations(nextSequenceCount: map<string, nat>, m: map<Variable, SVar>, declMap: DeclMappings)
+  {
+    static function Empty(declMap: DeclMappings): Incarnations {
+      Incarnations(map[], map[], declMap)
+    }
+
+    function Type2SType(typ: Type): SType {
+      declMap.Type2SType(typ)
+    }
+
+    function Variables(): set<Variable> {
+      m.Keys
+    }
+
+    // `Set` is intended to be used only during custom initializations of an Incarnations.
+    function Set(v: Variable, sv: SVar): Incarnations {
+      this.(nextSequenceCount := map[v.name := 0] + nextSequenceCount, m := m[v := sv])
+    }
+
+    method Update(v: Variable) returns (incarnations: Incarnations, x: SVar) {
+      var name := v.name;
+      var nextSequenceNumber;
+      if name in nextSequenceCount.Keys {
+        var n := nextSequenceCount[name];
+        name := name + "%" + Int2String(n);
+        nextSequenceNumber := n + 1;
+      } else {
+        nextSequenceNumber := 0;
+      }
+      x := new SVar(name, declMap.Type2SType(v.typ));
+      incarnations := this.(nextSequenceCount := nextSequenceCount[v.name := nextSequenceNumber], m := m[v := x]);
+    }
+
+    function DomainRestrict(variables: set<Variable>): Incarnations {
+      var m' := map v <- m.Keys | v in variables :: m[v];
+      this.(m := m')
+    }
+
+    // Create SVar's for the bound variables in "expr" and then substitute these and the other incarnations
+    // into "expr".
+    method REval(expr: Expr) returns (r: RSolvers.RExpr)
+      requires expr.WellFormed()
+    {
+      // TODO: handle bound variables
+      r := Substitute(expr);
+    }
+
+    function Substitute(expr: Expr): RSolvers.RExpr
+      requires expr.WellFormed()
+    {
+      match expr
+      case BLiteral(value) => RExpr.Boolean(value)
+      case ILiteral(value) => RExpr.Integer(value)
+      case CustomLiteral(s, typ) => RExpr.CustomLiteral(s, declMap.Type2SType(typ))
+      case IdExpr(v) =>
+        assume {:axiom} v in m;
+        // TODO: it would be nice to be able to keep the original variable if there's no incarnation; that would be the case for the bound variable in a let expression or quantifier
+        RExpr.Id(m[v])
+      case OperatorExpr(op, args) =>
+        var rArgs := SubstituteList(args);
+        match op {
+          case IfThenElse =>
+            RExpr.IfThenElse(rArgs[0], rArgs[1], rArgs[2])
+          case Neq =>
+            var eq := RExpr.FuncAppl(RExpr.Operator2ROperator(Operator.Eq), rArgs);
+            RExpr.FuncAppl(RExpr.Operator2ROperator(Operator.LogicalNot), [eq])
+          case _ =>
+            RExpr.FuncAppl(RExpr.Operator2ROperator(op), rArgs)
+        }
+      case FunctionCallExpr(func, args) =>
+        var rArgs := SubstituteList(args);
+        assume {:axiom} func in declMap.functionMap;
+        RExpr.FuncAppl(RSolvers.UserDefinedFunction(declMap.functionMap[func]), rArgs)
+      case LabeledExpr(_, body) =>
+        // TODO: do something with the label
+        Substitute(body)
+      case LetExpr(v, rhs, body) =>
+        RExpr.Boolean(true) //RExpr.LetExpr(v, Substitute(rhs), Substitute(body)) // TODO: this requires RExpr and Expr have the same Variables.
+      case QuantifierExpr(univ, v, patterns, body) =>
+        var trs := SubstitutePatterns(patterns);
+        var b := Substitute(body);
+        RExpr.Boolean(true) //RExpr.QuantifierExpr(univ, v, trs, b) // TODO: this requires RExpr and Expr have the same Variables.
+    }
+
+    function SubstituteList(exprs: seq<Expr>): seq<RSolvers.RExpr>
+      requires forall expr <- exprs :: expr.WellFormed()
+      ensures |SubstituteList(exprs)| == |exprs|
+    {
+      if exprs == [] then
+        []
+      else
+        [Substitute(exprs[0])] + SubstituteList(exprs[1..])
+    }
+
+    function SubstitutePatterns(patterns: seq<Pattern>): seq<seq<RSolvers.RExpr>>
+      requires forall tr <- patterns :: tr.WellFormed()
+    {
+      if patterns == [] then
+        []
+      else
+        assert patterns[0].WellFormed();
+        [SubstituteList(patterns[0].exprs)] + SubstitutePatterns(patterns[1..])
+    }
+  }
+
+}
